\documentclass{article}

\title{Introduction to Linear Algebra}
\author{Sam Wang}
\date{Oct 22, 2017}			
  
\usepackage{amsmath}

\newcommand{\site}[2][protocol]{\texttt{#1://#2}}
\newcommand{\fullref}[1]{\ref{#1} on page~\pageref{#1}}

\begin{document}

\maketitle
\tableofcontents

\section{Vector}

Definition
\begin{align}
  v &= \begin{bmatrix}v1\\ v2\\ v3\end{bmatrix}\\
  w &= \begin{bmatrix}w1\\ w2\\ w3\end{bmatrix}
\end{align}

Linear combination
\(cv + dw = \begin{bmatrix}
  c\cdot v1+d\cdot w1\\ 
  c\cdot v2+d\cdot w2\\ 
  c\cdot v3+d\cdot w3
  \end{bmatrix} \)

Dot(inner) product:
\( v\cdot w = v1\cdot w1 + v2\cdot w2 + v3\cdot w3 \)

Length:
\( \left \| v \right \| = \sqrt {v\cdot v} = \sqrt { {v_{1}}^{2} + {v_{2}}^{2} + {v_{3}}^{2} } \)

Unit vector:
\( u = \frac {v}{\left \| v \right \|} \)

Perpendicular vectors
\begin{align}
{\left \| v \right \|}^{2} + {\left \| w \right \|}^{2} &= {\left \| v - w \right \|}^{2}\\
(v_{1}^{2} + v_{2}^{2}) + ( w_{1}^{2} + w_{2}^{2}) &= {(v_{1} - w_{1})}^{2} + {(v_{2} - w_{2})}^{2}\\
v_{1}w_{1} + v_{2}w_{2} &= 0
\end{align}

Angle between vectors
\begin{equation}
u=\begin{bmatrix}
\cos \beta \\ 
\sin \beta
\end{bmatrix}
\\ U=\begin{bmatrix}
\cos \alpha  \\ 
\sin \alpha
\end{bmatrix}
\\ u\cdot U = \cos \alpha \cos \beta + \sin \alpha \sin \beta = \cos {\beta - \alpha} = \cos \theta = \frac {v\cdot w}{\left \| v \right \|\left \| w \right \|}
\\ because \cos \theta \leq 1
\\ therefore \left | v \cdot w \right | \leq \left \| v \right \| \left \| w \right \|
\\ therefore \left \| v+w \right \| \leq \left \| v \right \| + \left \| w \right \|
\end{equation}
06
\begin{equation}
v=\begin{bmatrix}
a\\ 
b
\end{bmatrix}
w=\begin{bmatrix}
b\\ 
a
\end{bmatrix}
\\ v\cdot w = 2ab \leq \left \| v \right \| \left \| w \right \| = a^2 + b^2
\\ x = a^2, y = b^2
\\ \sqrt {xy} \leq \frac {x+y}2
\\ therefore geometric.mean \leq arithmetic.mean
\end{equation}

\end{document}
