\documentclass{article}

\begin{document}

\begin{section}{Vector}
  Definition
  \begin{equation}
  v = \begin{bmatrix}v1\\ v2\\ v3\end{bmatrix} 
  \\ w = \begin{bmatrix}w1\\ w2\\ w3\end{bmatrix}
  \end{equation}

  01
  \begin{equation}
  cv + dw = \begin{bmatrix}
    c\cdot v1+d\cdot w1\\ 
    c\cdot v2+d\cdot w2\\ 
    c\cdot v3+d\cdot w3
  \end{bmatrix}
  \end{equation}

  02
  \begin{equation}
  v\cdot w = v1\cdot w1 + v2\cdot w2 + v3\cdot w3
  \end{equation}

  03
  \begin{equation}
  \left \| v \right \| = \sqrt {v\cdot v} = \sqrt { {v_{1}}^{2} + {v_{2}}^{2} + {v_{3}}^{2} }
  \\ u = \frac {v}{\left \| v \right \|}
  \end{equation}

  04
  \begin{equation}
  {\left \| v \right \|}^{2} + {\left \| w \right \|}^{2} = {\left \| v - w \right \|}^{2}
  \\\rightarrow (v_{1}^{2} + v_{2}^{2}) + ( w_{1}^{2} + w_{2}^{2}) = {(v_{1} - w_{1})}^{2} + {(v_{2} - w_{2})}^{2}
  \\\rightarrow v_{1}w_{1} + v_{2}w_{2} = 0
  \end{equation}

  05
  \begin{equation}
  u=\begin{bmatrix}
  \cos \beta \\ 
  \sin \beta
  \end{bmatrix}

  \\ U=\begin{bmatrix}
  \cos \alpha  \\ 
  \sin \alpha
  \end{bmatrix}

  \\ u\cdot U = \cos \alpha \cos \beta + \sin \alpha \sin \beta = \cos {\beta - \alpha} = \cos \theta = \frac {v\cdot w}{\left \| v \right \|\left \| w \right \|}
  \\ \because \cos \theta \leq 1
  \\ \therefore \left | v \cdot w \right | \leq \left \| v \right \| \left \| w \right \|
  \\ \therefore \left \| v+w \right \| \leq \left \| v \right \| + \left \| w \right \|
  \end{equation}

  06
  \begin{equation}
  v=\begin{bmatrix}
  a\\ 
  b
  \end{bmatrix}

  \\ w=\begin{bmatrix}
  b\\ 
  a
  \end{bmatrix}

  \\ v\cdot w = 2ab \leq \left \| v \right \| \left \| w \right \| = a^2 + b^2
  \\ x = a^2, y = b^2
  \\ \sqrt {xy} \leq \frac {x+y}2
  \\ \therefore geometric.mean \leq arithmetic.mean
  \end{equation}

\end{document}